Shake/Incremental/Basic.lean
@@ -1,11 +1,153 @@
-import Shake.Incremental.Store
-namespace Incremental
-open Std (HashMap)
-variable
-  (ℭ : BuildConfig)
-  (J : Type) [Input ℭ J]
-  [BEq ℭ.I] [Hashable ℭ.I] [∀ i, Hashable (ℭ.V i)]
-  [BEq ℭ.Q] [Hashable ℭ.Q] [∀ q, Hashable (ℭ.R q)]
-def run (tasks : Tasks ℭ) (ι₀ : ∀ i, ℭ.V i) (q₀ : ℭ.Q) : IO (ℭ.R q₀) := do
-  pure (compute tasks ι₀ q₀)
-end Incremental
+module
+
+public import Shake.Incremental
+
+@[expose] public section
+
+namespace Shake.Incremental
+
+variable (ℭ : BuildConfig) [BEq ℭ.I] [Hashable ℭ.I] [BEq ℭ.Q] [Hashable ℭ.Q] [∀ q, Hashable (ℭ.R q)]
+
+inductive FM (ℭ : BuildConfig) (q₀ : ℭ.Q) (α : Type) : Type
+  | pure (a : α) : FM ℭ q₀ α
+  | input (i : ℭ.I) (k : ℭ.V i → FM ℭ q₀ α) : FM ℭ q₀ α
+  | fetch (q : ℭ.Q) (hq : ℭ.rel q q₀) (k : ℭ.R q → FM ℭ q₀ α) : FM ℭ q₀ α
+
+namespace FM
+
+variable {ℭ : BuildConfig} {q₀ : ℭ.Q}
+
+def bind {α β : Type} (fa : FM ℭ q₀ α) (k : α → FM ℭ q₀ β) : FM ℭ q₀ β :=
+  match fa with
+  | pure a => k a
+  | input i kt => input i (fun v => bind (kt v) k)
+  | fetch q hq kt => fetch q hq (fun r => bind (kt r) k)
+
+instance : Monad (FM ℭ q₀) where
+  pure := pure
+  bind := bind
+
+instance : LawfulMonad (FM ℭ q₀) := LawfulMonad.mk'
+  (id_map := fun x => by induction x with
+    | pure _ => rfl
+    | input i kt ih => exact congrArg (input i) (funext ih)
+    | fetch q hq kt ih => exact congrArg (fetch q hq) (funext ih))
+  (pure_bind := fun _ _ => rfl)
+  (bind_assoc := fun x _ _ => by induction x with
+    | pure _ => rfl
+    | input i kt ih => exact congrArg (input i) (funext ih)
+    | fetch q hq kt ih => exact congrArg (fetch q hq) (funext ih))
+  (map_const := fun _ _ => rfl)
+  (seqLeft_eq := fun _ _ => rfl)
+  (seqRight_eq := fun _ _ => rfl)
+  (bind_pure_comp := fun _ _ => rfl)
+  (bind_map := fun _ _ => rfl)
+
+def evalTree {α : Type} (ι : ∀ i, ℭ.V i) (rec : ∀ q, ℭ.R q) : FM ℭ q₀ α → α
+  | pure a => a
+  | input i k => evalTree ι rec (k (ι i))
+  | fetch q _ k => evalTree ι rec (k (rec q))
+
+theorem evalTree_bind {α β : Type} (ι : ∀ i, ℭ.V i) (rec : ∀ q, ℭ.R q) (ma : FM ℭ q₀ α) (ka : α → FM ℭ q₀ β) :
+  evalTree ι rec (bind ma ka) = evalTree ι rec (ka (evalTree ι rec ma)) := by
+  induction ma with
+  | pure a => rfl
+  | input i kt ih => exact ih (ι i)
+  | fetch q _ kt ih => exact ih (rec q)
+
+abbrev pureInput (i : ℭ.I) : FM ℭ q₀ (ℭ.V i) := input i pure
+
+abbrev pureFetch (q : ℭ.Q) (hq : ℭ.rel q q₀) : FM ℭ q₀ (ℭ.R q) := fetch q hq pure
+
+end FM
+
+structure InputEntry (ℭ : BuildConfig) where
+  i : ℭ.I
+  v : ℭ.V i
+
+structure DepEntry (ℭ : BuildConfig) (q₀ : ℭ.Q) where
+  q : ℭ.Q
+  hq : ℭ.rel q q₀
+  r : ℭ.R q
+
+namespace FM
+
+variable {ℭ : BuildConfig} {q₀ : ℭ.Q}
+
+def evalTrace_inputs {α : Type} (ι : ∀ i, ℭ.V i) (rec : ∀ q, ℭ.R q) : FM ℭ q₀ α → List (InputEntry ℭ)
+  | pure _ => []
+  | input i k => ⟨i, ι i⟩ :: evalTrace_inputs ι rec (k (ι i))
+  | fetch q _ k => evalTrace_inputs ι rec (k (rec q))
+
+def evalTrace_deps {α : Type} (ι : ∀ i, ℭ.V i) (rec : ∀ q, ℭ.R q) : FM ℭ q₀ α → List (DepEntry ℭ q₀)
+  | pure _ => []
+  | input i k => evalTrace_deps ι rec (k (ι i))
+  | fetch q hq k => ⟨q, hq, rec q⟩ :: evalTrace_deps ι rec (k (rec q))
+
+theorem evalTrace_inputs_bind {α β : Type} (ι : ∀ i, ℭ.V i) (rec : ∀ q, ℭ.R q) (ma : FM ℭ q₀ α) (ka : α → FM ℭ q₀ β) :
+  evalTrace_inputs ι rec (bind ma ka) = evalTrace_inputs ι rec ma ++ evalTrace_inputs ι rec (ka (evalTree ι rec ma)) := by
+  induction ma with
+  | pure a => rfl
+  | input i kt ih => exact congrArg _ (ih (ι i))
+  | fetch q _ kt ih => exact ih (rec q)
+
+theorem evalTrace_deps_bind {α β : Type} (ι : ∀ i, ℭ.V i) (rec : ∀ q, ℭ.R q) (ma : FM ℭ q₀ α) (ka : α → FM ℭ q₀ β) :
+  evalTrace_deps ι rec (bind ma ka) = evalTrace_deps ι rec ma ++ evalTrace_deps ι rec (ka (evalTree ι rec ma)) := by
+  induction ma with
+  | pure a => rfl
+  | input i kt ih => exact ih (ι i)
+  | fetch q hq kt ih => exact congrArg _ (ih (rec q))
+
+theorem evalTrace_deps_value {α : Type} (ι : ∀ i, ℭ.V i) (rec : ∀ q, ℭ.R q) (t : FM ℭ q₀ α) :
+  ∀ p ∈ evalTrace_deps ι rec t, p.r = rec p.q := by
+  induction t with
+  | pure _ => nofun
+  | input i k ih => exact ih (ι i)
+  | fetch q hq k ih =>
+    exact fun
+    | _, .head _ => rfl
+    | p, .tail _ ht => ih (rec q) p ht
+
+theorem evalTree_cross {α : Type} (ι ι' : ∀ i, ℭ.V i) (rec rec' : ∀ q, ℭ.R q) (t : FM ℭ q₀ α)
+    (hin : ∀ p ∈ evalTrace_inputs ι rec t, ι' p.i = p.v)
+    (hdep : ∀ p ∈ evalTrace_deps ι rec t, rec' p.q = p.r) :
+    evalTree ι rec t = evalTree ι' rec' t := by
+  induction t with
+  | pure a => rfl
+  | input i k ih =>
+    show evalTree ι rec (k (ι i)) = evalTree ι' rec' (k (ι' i))
+    rw [hin ⟨i, ι i⟩ (.head _)]
+    exact ih (ι i) (fun p hp => hin p (.tail _ hp)) hdep
+  | fetch q hq k ih =>
+    show evalTree ι rec (k (rec q)) = evalTree ι' rec' (k (rec' q))
+    rw [hdep ⟨q, hq, rec q⟩ (.head _)]
+    exact ih (rec q) hin (fun p hp => hdep p (.tail _ hp))
+
+def evalAction (ι : ∀ i, ℭ.V i) (rec : ∀ q, ℭ.R q) : MonadAction (FM ℭ q₀) Id where
+  rel R t a := R (evalTree ι rec t) a
+  rel_pure hab := hab
+  rel_bind {_ _ _ _ _ _ ma _ ka _} hma hk := evalTree_bind ι rec ma ka ▸ hk _ _ hma
+
+end FM
+
+variable (ℭ : BuildConfig)
+
+def tasksTree (tasks : Tasks ℭ) (q₀ : ℭ.Q) : FM ℭ q₀ (ℭ.R q₀) :=
+  (tasks q₀).fn (FM ℭ q₀) FM.pureInput FM.pureFetch
+
+theorem tasksTree_eval (tasks : Tasks ℭ) (q₀ : ℭ.Q) (ι : ∀ i, ℭ.V i) (rec : ∀ q, ℭ.R q) :
+    FM.evalTree ι rec (tasksTree ℭ tasks q₀) = (tasks q₀).fn Id ι (fun q _ => rec q) :=
+  (tasks q₀).param (FM.evalAction ι rec) FM.pureFetch _ (fun _ => rfl) (fun _ _ => rfl)
+
+theorem tasksTree_eval_compute (tasks : Tasks ℭ) (q₀ : ℭ.Q) (ι : ∀ i, ℭ.V i) :
+    FM.evalTree ι (compute tasks ι) (tasksTree ℭ tasks q₀) = compute tasks ι q₀ := by
+  rw [tasksTree_eval]
+  conv => rhs; unfold compute
+
+theorem compute_cross (tasks : Tasks ℭ) (q₀ : ℭ.Q) (ι ι' : ∀ i, ℭ.V i)
+    (hin : ∀ p ∈ FM.evalTrace_inputs ι (compute tasks ι) (tasksTree ℭ tasks q₀), ι' p.i = p.v)
+    (hdep : ∀ p ∈ FM.evalTrace_deps ι (compute tasks ι) (tasksTree ℭ tasks q₀), compute tasks ι' p.q = p.r) :
+    compute tasks ι q₀ = compute tasks ι' q₀ := by
+  rw [← tasksTree_eval_compute ℭ tasks q₀ ι, FM.evalTree_cross ι ι' _ _ _ hin hdep, tasksTree_eval_compute ℭ tasks q₀ ι']
+
+end Shake.Incremental
