Shake.lean
@@ -1,0 +1,4 @@
+module
+
+public import Shake.Development
+public import Shake.Incremental
