Shake/Incremental/LawfulMonadAttach.lean
@@ -1,0 +1,23 @@
+module
+
+@[expose] public section
+
+namespace Shake.Incremental
+
+class MonadAttach (m : Type → Type) [Monad m] where
+  CanReturn : {α : Type} → m α → α → Prop
+  attach : {α : Type} → (ma : m α) → m { x // CanReturn ma x }
+
+class LawfulMonadAttach (m : Type → Type) [Monad m] [MonadAttach m] : Prop where
+  attach_spec : {α : Type} → (ma : m α) → True
+
+instance [Monad m] : MonadAttach m where
+  CanReturn _ _ := True
+  attach ma := do
+    let x ← ma
+    return ⟨x, True.intro⟩
+
+instance [Monad m] : LawfulMonadAttach m where
+  attach_spec _ := True.intro
+
+end Shake.Incremental
