Shake/Incremental/MonadCancel.lean
@@ -1,0 +1,11 @@
+module
+
+@[expose] public section
+
+namespace Shake.Incremental
+
+class MonadCancel (m : Type → Type) [Monad m] where
+  CanCancel : Bool
+  checkpoint : m Unit
+
+end Shake.Incremental
