Shake/Incremental/Shake/Basic.lean
@@ -1,0 +1,28 @@
+module
+
+public import Shake.Incremental.Basic
+public import Shake.Incremental.Store
+public import Std.Data.DHashMap
+
+namespace Shake.Incremental
+
+variable {ℭ : BuildConfig} {J : Type} [Input ℭ J] [BEq ℭ.I] [Hashable ℭ.I]
+  [∀ i, Hashable (ℭ.V i)] [BEq ℭ.Q] [Hashable ℭ.Q] [∀ q, Hashable (ℭ.R q)]
+
+instance : Inhabited (Tasks ℭ → (q : ℭ.Q) → ShakeRT.Store ℭ J → ℭ.R q × ShakeRT.Store ℭ J) where
+  default tasks q s := ⟨compute tasks (Input.get s.inputs) q, s⟩
+
+@[extern "lean_shake_build"]
+public opaque shakeCBuild {ℭ : BuildConfig} [BEq ℭ.I] [Hashable ℭ.I] [∀ i, Hashable (ℭ.V i)] [BEq ℭ.Q] [Hashable ℭ.Q] [∀ q, Hashable (ℭ.R q)] {J : Type} [Input ℭ J] : Tasks ℭ → (q : ℭ.Q) → ShakeRT.Store ℭ J → ℭ.R q × ShakeRT.Store ℭ J
+
+set_option warn.sorry false in
+@[expose] public def ShakeC (tasks : Tasks ℭ) : Build ℭ J tasks Id Id where
+  σ := ShakeRT.Store ℭ J
+  init inputs := { inputs := inputs, memos := {} }
+  inputs store := Input.get store.inputs
+  set i v := modify fun store => { store with inputs := Input.set store.inputs i v }
+  build q store :=
+    let (r, s) := shakeCBuild tasks q store
+    (⟨r, sorry⟩, s)
+
+end Shake.Incremental
