Shake/Internal/Core/Storage.lean
@@ -1,0 +1,43 @@
+module
+
+public import Shake.Incremental
+public import Shake.Internal.Core.Binary
+public import Shake.Incremental.Store
+public import Std.Data.HashMap
+
+@[expose] public section
+
+namespace Shake.Internal.Core
+
+open Shake.Incremental (BuildConfig)
+open Shake.Incremental.ShakeRT
+
+public structure Storage where
+  version : String := "SHAKE-LEAN-0.1"
+  path : String
+
+section
+  variable (ℭ : BuildConfig) {J : Type}
+    [BEq ℭ.Q] [Hashable ℭ.Q] [BEq ℭ.I] [Hashable ℭ.I]
+    [Binary J] [Binary ℭ.Q] [Binary ℭ.I] [∀ q, Binary (ℭ.R q)]
+
+  public def saveStore (storage : Storage) (s : Store ℭ J) : IO Unit := do
+    let content := serializeStore s
+    let fullData := Binary.put storage.version ++ content
+    IO.FS.writeBinFile storage.path fullData
+
+  public def loadStore (storage : Storage) : IO (Option (Store ℭ J)) := do
+    if ← System.FilePath.pathExists storage.path then
+      let data ← IO.FS.readBinFile storage.path
+      match Binary.get (α := String) data with
+      | some (v, rest) =>
+        if v == storage.version then
+          match deserializeStore (ℭ := ℭ) rest with
+          | some (s, _) => return some s
+          | none => return none
+        else return none
+      | none => return none
+    else return none
+end
+
+end Shake.Internal.Core
